Cfg.dfy
@@ -7,7 +7,7 @@ module BoogieCfg {
   import opened BoogieSemantics
   import opened Wrappers
 
-  type BasicBlock = seq<SimpleCmd>
+  type BasicBlock = SimpleCmd
   type BlockId = nat 
 
   datatype Cfg = Cfg(entry: BlockId, blocks: map<BlockId, BasicBlock>, successors: map<BlockId, seq<BlockId>>)
@@ -20,50 +20,692 @@ module BoogieCfg {
       (forall i :: 0 <= i < |g.successors[blockId]| ==> g.successors[blockId][i] in g.blocks.Keys))
   }
 
-  function IsAcyclicSeq(g: Cfg, ns: seq<BlockId>, cover: set<BlockId>) : bool
-    requires CfgWf(g)
-    requires (forall i :: 0 <= i < |ns| ==> ns[i] in g.blocks.Keys)
+  type SuccessorRel = map<BlockId, seq<BlockId>>
+
+  function IsAcyclicSeq(r: SuccessorRel, ns: seq<BlockId>, cover: set<BlockId>) : bool
     decreases cover, 1, ns
   {
-    if |ns| == 0 then true
-    else
-      IsAcyclic(g, ns[0], cover) && IsAcyclicSeq(g, ns[1..], cover)
+    |ns| != 0 ==> ( IsAcyclic(r, ns[0], cover) && IsAcyclicSeq(r, ns[1..], cover) )
   }
 
-  function IsAcyclic(g: Cfg, n: BlockId, cover: set<BlockId>) : bool
-    requires CfgWf(g)
-    requires n in g.blocks.Keys
+  function IsAcyclic(r: SuccessorRel, n: BlockId, cover: set<BlockId>) : bool
     decreases cover, 0
   {
-    (n in cover) && IsAcyclicSeq(g, g.successors[n], cover - {n})
+    n in r.Keys ==> ( n in cover && IsAcyclicSeq(r, r[n], cover - {n}) )
   }
 
-  function WpCfgConjunction<A(!new)>(a: absval_interp<A>, g: Cfg, ns: seq<BlockId>, post: Predicate<A>, cover: set<BlockId>) : Predicate<A>
-    requires CfgWf(g)
-    requires (forall i :: 0 <= i < |ns| ==> ns[i] in g.blocks.Keys)
-    requires IsAcyclicSeq(g, ns, cover)
+  function BasicBlockToCmd(block: BasicBlock) : Cmd
+  {
+    SimpleCmd(block)
+  }
+
+  /*=================== Wp semantics ==========================================*/
+  datatype WpPostCfg<!A> = WpPostCfg(normal: Predicate<A>, exceptional: map<BlockId, Predicate<A>>)
+
+  function WpCfgConjunction<A(!new)>(
+    a: absval_interp<A>, 
+    g: Cfg, 
+    ns: seq<BlockId>, 
+    post: Predicate<A>, 
+    cover: set<BlockId>) : Predicate<A>
+    requires g.successors.Keys <= g.blocks.Keys //not being in the domain of the successor relation is the same as not having any successors
+    requires |ns| >= 1
     decreases cover, 1, ns
-  { s =>
-      if |ns| == 0 then Some(true)
+  {   //this definition allows one to deduce that WpCfgConjunction and WpCfg coincide for singleton sequences (instead of just being pointwise equal)
+      if |ns| == 1 then WpCfg(a, g, ns[0], post, cover) 
       else 
-        assert ns[0] in g.blocks.Keys;
-        var res1 :- WpCfg(a, g, ns[0], post, cover)(s);
-        var res2 :- WpCfgConjunction(a, g, ns[1..], post, cover)(s);
-        Some(res1 && res2)
+        s => 
+          var res1 :- WpCfg(a, g, ns[0], post, cover)(s);
+          var res2 :- WpCfgConjunction(a, g, ns[1..], post, cover)(s);
+          Some(res1 && res2)
   }
 
   function WpCfg<A(!new)>(a: absval_interp<A>, g: Cfg, n: BlockId, post: Predicate<A>, cover: set<BlockId>) : Predicate<A>
-    requires CfgWf(g)
-    requires n in g.blocks.Keys
-    requires IsAcyclic(g, n, cover)
+    requires g.successors.Keys <= g.blocks.Keys //not being in the domain of the successor relation is the same as not having any successors
     decreases cover, 0
   {
-    var successors := g.successors[n];
-
-    if |successors| == 0 then 
-      WpShallowSimpleCmdConj(a, g.blocks[n], post)
+    if IsAcyclic(g.successors, n, cover) then
+      if n !in g.blocks.Keys then
+        post
+      else 
+        var successors := if n in g.successors.Keys then g.successors[n] else [];
+        if |successors| == 0 then 
+          WpShallowSimpleCmd(a, g.blocks[n], post)
+        else 
+          WpShallowSimpleCmd(a, g.blocks[n], WpCfgConjunction(a, g, successors, post, cover - {n}))
     else 
-      WpShallowSimpleCmdConj(a, g.blocks[n], WpCfgConjunction(a, g, successors, post, cover - {n}))
+      s => None
   }
 
+  lemma {:verify false} WpCfgConjunctionPointwise<A(!new)>(a: absval_interp<A>, g: Cfg, ns: seq<BlockId>, post1: Predicate<A>, post2: Predicate<A>, cover: set<BlockId>, s: state<A>) 
+    requires g.successors.Keys <= g.blocks.Keys //not being in the domain of the successor relation is the same as not having any successors
+    //requires IsAcyclicSeq(g.successors, ns, cover)
+    requires (forall s :: post1(s) == post2(s))
+    requires |ns| >= 1
+    ensures WpCfgConjunction(a, g, ns, post1, cover)(s) == WpCfgConjunction(a, g, ns, post2, cover)(s)
+    decreases cover, 1, ns
+  {
+    WpCfgPointwise(a, g, ns[0], post1, post2, cover, s);
+    if |ns| > 1 {
+      WpCfgConjunctionPointwise(a, g, ns[1..], post1, post2, cover, s);
+    }
+  }
+
+  lemma {:verify false} WpCfgPointwise<A(!new)>(a: absval_interp<A>, g: Cfg, n: BlockId, post1: Predicate<A>, post2: Predicate<A>, cover: set<BlockId>, s: state<A>)
+    requires g.successors.Keys <= g.blocks.Keys //not being in the domain of the successor relation is the same as not having any successors
+    //requires IsAcyclic(g.successors, n, cover)
+    requires (forall s :: post1(s) == post2(s))
+    ensures WpCfg(a, g, n, post1, cover)(s) == WpCfg(a, g, n, post2, cover)(s)
+    decreases cover, 0
+  {
+    if IsAcyclic(g.successors, n, cover) {
+      if n in g.blocks.Keys {
+        var block := g.blocks[n];
+        var successors := if n in g.successors.Keys then g.successors[n] else [];
+        if |successors| == 0  {
+          WpShallowSimpleCmdPointwise(a, block, post1, post2, s);
+        } else {
+          var successorPost1 := WpCfgConjunction(a, g, successors, post1, cover - {n});
+          var successorPost2 := WpCfgConjunction(a, g, successors, post2, cover - {n});
+          
+          forall s' | true
+            ensures successorPost1(s') == successorPost2(s')
+          {
+            WpCfgConjunctionPointwise(a, g, successors, post1, post2, cover - {n}, s');
+          }
+          WpShallowSimpleCmdPointwise(a, block, successorPost1, successorPost2, s);
+        }
+      }
+    }
+  }
+
+  lemma {:verify false} WpCfgConjunctionEntryIndep<A(!new)>(a: absval_interp<A>, cfg: Cfg, entryOther: BlockId, ns: seq<BlockId>, post: Predicate<A>, cover: set<BlockId>)
+    requires |ns| > 0
+    requires cfg.successors.Keys <= cfg.blocks.Keys
+    ensures WpCfgConjunction(a, cfg, ns, post, cover) == WpCfgConjunction(a, Cfg(entryOther, cfg.blocks, cfg.successors), ns, post, cover)
+    decreases cover, 1, |ns|
+  {
+    WpCfgEntryIndep(a, cfg, entryOther, ns[0], post, cover);
+  }
+  
+  lemma {:verify false} WpCfgEntryIndep<A(!new)>(a: absval_interp<A>, cfg: Cfg, entryOther: BlockId, n: BlockId, post: Predicate<A>, cover: set<BlockId>)
+    requires cfg.successors.Keys <= cfg.blocks.Keys
+    ensures WpCfg(a, cfg, n, post, cover) == WpCfg(a, Cfg(entryOther, cfg.blocks, cfg.successors), n, post, cover)
+    decreases cover, 0
+  {
+    var successors := if n in cfg.successors.Keys then cfg.successors[n] else [];
+
+    if IsAcyclic(cfg.successors, n, cover) {
+      if |successors| > 0 {
+        WpCfgConjunctionEntryIndep(a, cfg, entryOther, successors, post, cover - {n});
+      }
+    }  
+  }
+
+  /*======================Acyclicity lemma {:verify false}s ===================================*/
+
+  lemma {:verify false} IsAcyclicSeqForall(r: SuccessorRel, ns: seq<BlockId>, cover: set<BlockId>)
+    requires IsAcyclicSeq(r, ns, cover)
+    ensures forall n :: n in ns ==> IsAcyclic(r, n, cover)
+  { }
+
+  lemma {:verify false} IsAcyclicElem(r: SuccessorRel, ns: seq<BlockId>, nSucc: BlockId, cover: set<BlockId>)
+    requires IsAcyclicSeq(r, ns, cover)
+    requires nSucc in ns
+    ensures IsAcyclic(r, nSucc, cover)
+  { }
+
+  lemma {:verify false} IsAcyclicSeqLargerCover(r: SuccessorRel, ns: seq<BlockId>, cover1: set<BlockId>, cover2: set<BlockId>)
+    requires cover1 <= cover2 && IsAcyclicSeq(r, ns, cover1)
+    ensures IsAcyclicSeq(r, ns, cover2)
+    decreases cover1, 1, ns
+  {
+    if |ns| != 0 {
+      IsAcyclicLargerCover(r, ns[0], cover1, cover2); 
+      IsAcyclicSeqLargerCover(r, ns[1..], cover1, cover2);
+    }
+  }
+
+  lemma {:verify false} IsAcyclicLargerCover(r: SuccessorRel, n: BlockId, cover1: set<BlockId>, cover2: set<BlockId>)
+    requires cover1 <= cover2 && IsAcyclic(r, n, cover1)
+    ensures IsAcyclic(r, n, cover2)
+    decreases cover1, 0
+  {
+    if n in r.Keys {
+      IsAcyclicSeqLargerCover(r, r[n], cover1 - {n}, cover2 - {n});
+    }
+  }
+
+  lemma {:verify false} IsAcyclicSeqMerge(
+    r1: SuccessorRel, 
+    r2: SuccessorRel, 
+    ns1: seq<BlockId>,
+    n2Entry: BlockId,
+    cover1: set<BlockId>, 
+    cover2: set<BlockId>)
+    requires cover1 !! cover2
+    requires r1.Keys !! r2.Keys
+    requires IsAcyclicSeq(r1, ns1, cover1)
+    requires IsAcyclic(r2, n2Entry, cover2)
+
+    requires 
+      (forall i :: 0 <= i < |ns1| ==> 
+             ns1[i] in r1.Keys || ns1[i] == n2Entry)
+
+    requires !(n2Entry in r1.Keys)
+
+    requires 
+      (forall i :: 0 <= i < |ns1| ==> 
+             ns1[i] in r1.Keys || ns1[i] == n2Entry)
+    // successors in r1 are either n2Entry or blocks recorded in r1
+    requires 
+      forall n1 :: n1 in r1.Keys ==>   
+        (forall i :: 0 <= i < |r1[n1]| ==> (r1[n1][i] == n2Entry || r1[n1][i] in r1.Keys))
+
+    // successors in r2 are not recorded in r1
+    requires
+      forall n2 :: n2 in r2.Keys ==>   
+        (forall i :: 0 <= i < |r2[n2]| ==> !(r2[n2][i] in r1.Keys))
+    ensures IsAcyclicSeq(r1 + r2, ns1, cover1 + cover2)
+    decreases cover1, 1, ns1
+  {
+    if |ns1| != 0 {
+      IsAcyclicMerge(r1, r2, ns1[0], n2Entry, cover1, cover2);
+      IsAcyclicSeqMerge(r1, r2, ns1[1..], n2Entry, cover1, cover2);
+    }
+  }
+
+  lemma {:verify false} IsAcyclicMerge(
+    r1: SuccessorRel, 
+    r2: SuccessorRel, 
+    n1Entry: BlockId,
+    n2Entry: BlockId,
+    cover1: set<BlockId>, 
+    cover2: set<BlockId>)
+    requires cover1 !! cover2
+    requires r1.Keys !! r2.Keys
+    requires IsAcyclic(r1, n1Entry, cover1)
+    requires IsAcyclic(r2, n2Entry, cover2)
+
+    requires n1Entry in r1.Keys || n1Entry == n2Entry
+    requires !(n2Entry in r1.Keys)
+
+    // successors in r1 are either n2Entry or blocks recorded in r1
+    requires 
+      forall n1 :: n1 in r1.Keys ==>   
+        (forall i :: 0 <= i < |r1[n1]| ==> (r1[n1][i] == n2Entry || r1[n1][i] in r1.Keys))
+
+    // successors in r2 are not recorded in r1
+    requires
+      forall n2 :: n2 in r2.Keys ==>   
+        (forall i :: 0 <= i < |r2[n2]| ==> !(r2[n2][i] in r1.Keys))
+    ensures IsAcyclic(r1 + r2, n1Entry, cover1 + cover2)
+    decreases cover1, 0
+  {
+    if n1Entry in r1.Keys {
+      IsAcyclicSeqMerge(r1, r2, r1[n1Entry], n2Entry, cover1 - {n1Entry}, cover2);
+      calc {
+        IsAcyclicSeq(r1 + r2, r1[n1Entry], (cover1 - {n1Entry}) + cover2); 
+      == { assert (cover1 - {n1Entry}) + cover2 == (cover1 + cover2) - {n1Entry}; }
+        IsAcyclicSeq(r1 + r2, r1[n1Entry], (cover1 + cover2) - {n1Entry});
+      }
+    } else {
+      IsAcyclicExtend(r1, r2, n2Entry, cover2);
+      IsAcyclicLargerCover(r1+r2, n2Entry, cover2, cover1 + cover2);
+    }
+  }
+
+  lemma {:verify false} WpCfgConjunctionMerge<A(!new)>(
+    a: absval_interp<A>, 
+    g1: Cfg,
+    g2: Cfg,
+    ns: seq<BlockId>,
+    exit1: BlockId, 
+    post: Predicate<A>, 
+    cover1: set<BlockId>, 
+    cover2: set<BlockId>)
+    requires |ns| >= 1
+    requires g1.successors.Keys <= g1.blocks.Keys
+    requires g2.successors.Keys <= g2.blocks.Keys
+    requires exit1 in g1.blocks.Keys && exit1 !in g1.successors.Keys
+    requires g1.blocks.Keys !! g2.blocks.Keys
+    requires IsAcyclicSeq(g1.successors, ns, cover1)
+    requires IsAcyclic(g2.successors, g2.entry, cover2)
+    requires IsAcyclicSeq(g1.successors[exit1 := [g2.entry]] + g2.successors, ns, cover1+cover2+{exit1})
+
+    requires cover2 !! g1.blocks.Keys
+
+    requires !(g2.entry in g1.blocks.Keys)
+
+    // successors in g1.successors are either g2.entry or blocks recorded in g1.successors
+    requires 
+      forall n1 :: n1 in g1.successors.Keys ==>   
+        (forall i :: 0 <= i < |g1.successors[n1]| ==> (g1.successors[n1][i] in g1.successors.Keys || 
+                                                         g1.successors[n1][i] == exit1))
+
+    requires (forall n :: n in ns ==> n in g1.successors.Keys || n == exit1)
+    requires g2.entry != exit1
+
+    requires forall n1 :: n1 in g1.successors.Keys ==> g1.successors[n1] != []
+
+    // successors in g2.successors are not recorded in g1.blocks
+    requires
+      forall n2 :: n2 in g2.successors.Keys ==>   
+        (forall i :: 0 <= i < |g2.successors[n2]| ==> g2.successors[n2][i] !in g1.blocks.Keys)
+    ensures 
+      var successors' := (g1.successors[exit1 := [g2.entry]] + g2.successors);
+      var mergedCfg := Cfg(g1.entry, g1.blocks + g2.blocks, successors');
+      WpCfgConjunction(a, g1, ns, WpCfg(a, g2, g2.entry, post, cover2), cover1) ==
+      WpCfgConjunction(a, mergedCfg, ns, post, cover1+cover2+{exit1})
+    decreases cover1, 1, ns
+  {
+    WpCfgMerge(a, g1, g2, ns[0], exit1, post, cover1, cover2);
+  }
+
+  lemma {:verify false} WpCfgMerge<A(!new)>(
+    a: absval_interp<A>, 
+    g1: Cfg,
+    g2: Cfg,
+    g1Entry: BlockId,
+    exit1: BlockId, 
+    post: Predicate<A>, 
+    cover1: set<BlockId>, 
+    cover2: set<BlockId>)
+    requires g1.successors.Keys <= g1.blocks.Keys
+    requires g2.successors.Keys <= g2.blocks.Keys
+    requires exit1 in g1.blocks.Keys && exit1 !in g1.successors.Keys
+    requires g1.blocks.Keys !! g2.blocks.Keys
+    requires IsAcyclic(g1.successors, g1Entry, cover1)
+    requires IsAcyclic(g2.successors, g2.entry, cover2)
+    requires IsAcyclic(g1.successors[exit1 := [g2.entry]] + g2.successors, g1Entry, cover1+cover2+{exit1})
+
+    requires cover2 !! g1.blocks.Keys
+
+    requires !(g2.entry in g1.blocks.Keys)
+
+    // successors in g1.successors are either g2.entry or blocks recorded in g1.successors
+    requires 
+      forall n1 :: n1 in g1.successors.Keys ==>   
+        (forall i :: 0 <= i < |g1.successors[n1]| ==> (g1.successors[n1][i] in g1.successors.Keys || 
+                                                         g1.successors[n1][i] == exit1))
+
+    requires g1Entry in g1.successors.Keys || g1Entry == exit1
+    requires g2.entry != exit1
+
+    requires forall n1 :: n1 in g1.successors.Keys ==> g1.successors[n1] != []
+
+    // successors in g2.successors are not recorded in g1.blocks
+    requires
+      forall n2 :: n2 in g2.successors.Keys ==>   
+        (forall i :: 0 <= i < |g2.successors[n2]| ==> g2.successors[n2][i] !in g1.blocks.Keys)
+    ensures 
+      var successors' := (g1.successors[exit1 := [g2.entry]] + g2.successors);
+      var mergedCfg := Cfg(g1.entry, g1.blocks + g2.blocks, successors');
+      WpCfg(a, g1, g1Entry, WpCfg(a, g2, g2.entry, post, cover2), cover1) ==
+      WpCfg(a, mergedCfg, g1Entry, post, cover1+cover2+{exit1})
+    decreases cover1, 0
+    {
+      var cover3 := cover1+cover2+{exit1};
+      var block := g1.blocks[g1Entry];
+      var successors := if g1Entry in g1.successors.Keys then g1.successors[g1Entry] else [];
+
+      var successors' := (g1.successors[exit1 := [g2.entry]] + g2.successors);
+      var mergedCfg := Cfg(g1.entry, g1.blocks + g2.blocks, successors');
+
+      calc {
+        WpCfg(a, g2, g2.entry, post, cover2);
+          { WpCfgLargerCover(a, g2, g2.entry, post, cover2, cover3); }
+        WpCfg(a, g2, g2.entry, post, cover3);
+          { IsAcyclicLargerCover(g2.successors, g2.entry, cover2, cover3);
+
+            WpCfgExtend(a, mergedCfg, g2, g1.blocks, g1.successors[exit1 := [g2.entry]], g2.entry, post, cover3); }
+        WpCfg(a, mergedCfg, g2.entry, post, cover3);
+      }
+
+      if |successors| == 0 {
+        assert g1Entry == exit1;
+
+        calc {
+          WpCfg(a, mergedCfg, g1Entry, post, cover3);
+          WpShallowSimpleCmd(a, block, WpCfgConjunction(a, mergedCfg, [g2.entry], post, cover3 - {g1Entry}));
+          WpShallowSimpleCmd(a, block, WpCfg(a, mergedCfg, g2.entry, post, cover3 - {g1Entry})); 
+            { WpCfgLargerCover(a, mergedCfg, g2.entry, post, cover3 - {g1Entry}, cover3); }
+          WpShallowSimpleCmd(a, block, WpCfg(a, mergedCfg, g2.entry, post, cover3));
+            { assert WpCfg(a, mergedCfg, g2.entry, post, cover3) == WpCfg(a, g2, g2.entry, post, cover2); }
+          WpShallowSimpleCmd(a, block, WpCfg(a, g2, g2.entry, post, cover2));
+          WpCfg(a, g1, g1Entry, WpCfg(a, g2, g2.entry, post, cover2), cover1);
+        }
+      } else {
+        assert g1.blocks[g1Entry] == mergedCfg.blocks[g1Entry];
+        assert g1Entry != exit1;
+        calc {
+          WpCfg(a, mergedCfg, g1Entry, post, cover3);
+          WpShallowSimpleCmd(a, block, WpCfgConjunction(a, mergedCfg, successors, post, cover3-{g1Entry}));
+            { 
+              assert cover3-{g1Entry} == (cover1-{g1Entry})+cover2+{exit1};
+
+              WpCfgConjunctionMerge(a, g1, g2, successors, exit1, post, cover1-{g1Entry}, cover2);
+            }
+          WpShallowSimpleCmd(a, block, WpCfgConjunction(a, g1, successors, WpCfg(a, g2, g2.entry, post, cover2), cover1-{g1Entry}));
+          WpCfg(a, g1, g1Entry, WpCfg(a, g2, g2.entry, post, cover2), cover1);
+        }
+      }
+    }
+
+  
+  lemma {:verify false} WpCfgConjunctionLargerCover<A(!new)>(
+    a: absval_interp<A>, 
+    g: Cfg,
+    ns: seq<BlockId>,
+    post: Predicate<A>, 
+    cover1: set<BlockId>, 
+    cover2: set<BlockId>)
+  requires g.successors.Keys <= g.blocks.Keys
+  requires |ns| >= 1
+  requires cover1 <= cover2
+  requires IsAcyclicSeq(g.successors, ns, cover1)
+  ensures WpCfgConjunction(a, g, ns, post, cover1) == WpCfgConjunction(a, g, ns, post, cover2)
+  decreases cover1, 1, ns
+  {
+    WpCfgLargerCover(a, g, ns[0], post, cover1, cover2);
+  }
+
+  lemma {:verify false} WpCfgLargerCover<A(!new)>(
+    a: absval_interp<A>, 
+    g: Cfg,
+    n: BlockId,
+    post: Predicate<A>, 
+    cover1: set<BlockId>, 
+    cover2: set<BlockId>) 
+  requires g.successors.Keys <= g.blocks.Keys
+  requires cover1 <= cover2
+  requires IsAcyclic(g.successors, n, cover1)
+  ensures WpCfg(a, g, n, post, cover1) == WpCfg(a, g, n, post, cover2)
+  decreases cover1, 0
+  {
+    IsAcyclicLargerCover(g.successors, n, cover1, cover2);
+    
+    var successors := if n in g.successors.Keys then g.successors[n] else [];
+
+    if |successors| > 0 {
+      WpCfgConjunctionLargerCover(a, g, successors, post, cover1-{n}, cover2-{n});
+    }
+  }
+
+  lemma {:verify false} WpCfgConjunctionExtend<A(!new)>(a: absval_interp<A>, cfgMerged: Cfg, cfg2: Cfg, b1: map<BlockId, BasicBlock>, r1: SuccessorRel, ns: seq<BlockId>, post: Predicate<A>, cover: set<BlockId>)
+    requires 
+      var r2 := cfg2.successors;
+      && |ns| >= 1
+      && cfgMerged.successors == r1 + r2
+      && cfgMerged.blocks == b1 + cfg2.blocks
+      && r1.Keys !! r2.Keys
+      && b1.Keys !! cfg2.blocks.Keys
+      && cfgMerged.successors.Keys <= cfgMerged.blocks.Keys
+      && cfg2.successors.Keys <= cfg2.blocks.Keys
+      && IsAcyclicSeq(r2, ns, cover)
+      && r1.Keys <= b1.Keys
+      && (forall n :: n in ns ==> n !in b1.Keys)
+      && (forall n2 :: n2 in r2.Keys ==>   
+           (forall i :: 0 <= i < |r2[n2]| ==> r2[n2][i] !in b1))
+    ensures WpCfgConjunction(a, cfgMerged, ns, post, cover) == WpCfgConjunction(a, cfg2, ns, post, cover)
+    decreases cover, 1, ns
+  {
+    WpCfgExtend(a, cfgMerged, cfg2, b1, r1, ns[0], post, cover);
+  }
+
+  lemma {:verify false} WpCfgExtend2<A(!new)>(a: absval_interp<A>, cfgMerged: Cfg, cfg1: Cfg, b2: map<BlockId, BasicBlock>, r2: SuccessorRel, n1Entry: BlockId, post: Predicate<A>, cover: set<BlockId>)
+    requires 
+      var r1 := cfg1.successors;
+      && cfgMerged.successors == r1 + r2
+      && cfgMerged.blocks == cfg1.blocks + b2
+      && r1.Keys !! r2.Keys
+      && cfg1.blocks.Keys !! b2.Keys
+      && cfgMerged.successors.Keys <= cfgMerged.blocks.Keys
+      && cfg1.successors.Keys <= cfg1.blocks.Keys
+      && IsAcyclic(r1, n1Entry, cover)
+      && r2.Keys <= b2.Keys
+      && n1Entry !in b2.Keys   
+      && (forall n2 :: n2 in r1.Keys ==>   
+           (forall i :: 0 <= i < |r1[n2]| ==> r1[n2][i] !in b2.Keys))
+    ensures WpCfg(a, cfgMerged, n1Entry, post, cover) == WpCfg(a, cfg1, n1Entry, post, cover)
+  {
+    assert cfg1.successors + r2 == r2 + cfg1.successors;
+    assert cfg1.blocks + b2 == b2 + cfg1.blocks;
+    WpCfgExtend(a, cfgMerged, cfg1, b2, r2, n1Entry, post, cover);
+  }
+  
+  lemma {:verify false} WpCfgExtend<A(!new)>(a: absval_interp<A>, cfgMerged: Cfg, cfg2: Cfg, b1: map<BlockId, BasicBlock>, r1: SuccessorRel, n2Entry: BlockId, post: Predicate<A>, cover: set<BlockId>)
+    requires 
+      var r2 := cfg2.successors;
+      && cfgMerged.successors == r1 + r2
+      && cfgMerged.blocks == b1 + cfg2.blocks
+      && r1.Keys !! r2.Keys
+      && b1.Keys !! cfg2.blocks.Keys
+      && cfgMerged.successors.Keys <= cfgMerged.blocks.Keys
+      && cfg2.successors.Keys <= cfg2.blocks.Keys
+      && IsAcyclic(r2, n2Entry, cover)
+      && r1.Keys <= b1.Keys
+      && n2Entry !in b1.Keys   
+      && (forall n2 :: n2 in r2.Keys ==>   
+           (forall i :: 0 <= i < |r2[n2]| ==> r2[n2][i] !in b1.Keys))
+    ensures WpCfg(a, cfgMerged, n2Entry, post, cover) == WpCfg(a, cfg2, n2Entry, post, cover)
+    decreases cover, 0
+  {
+    var successors := if n2Entry in cfg2.successors.Keys then cfg2.successors[n2Entry] else [];
+    var successorsMerged := if n2Entry in cfgMerged.successors.Keys then cfgMerged.successors[n2Entry] else [];
+
+    assert successors == successorsMerged;
+
+    IsAcyclicExtend(r1, cfg2.successors, n2Entry, cover);
+    assert IsAcyclic(cfgMerged.successors, n2Entry, cover);
+
+    if n2Entry in cfg2.blocks.Keys {
+      var block := cfg2.blocks[n2Entry];
+      assert cfgMerged.blocks[n2Entry] == block;
+      assert n2Entry in cfgMerged.blocks.Keys;
+      if |successors| > 0 {
+        assert |successorsMerged| > 0;
+        WpCfgConjunctionExtend(a, cfgMerged, cfg2, b1, r1, successors, post, cover - {n2Entry});
+        calc {
+          WpCfg(a, cfg2, n2Entry, post, cover);
+          WpShallowSimpleCmd(a, block, WpCfgConjunction(a, cfg2, successors, post, cover-{n2Entry}));
+          WpShallowSimpleCmd(a, block, WpCfgConjunction(a, cfgMerged, successors, post, cover-{n2Entry}));
+          WpShallowSimpleCmd(a, block, WpCfgConjunction(a, cfgMerged, successorsMerged, post, cover-{n2Entry}));
+          WpCfg(a, cfgMerged, n2Entry, post, cover);
+        }
+      }
+    } 
+  }
+  /*
+  lemma {:verify false} IsAcyclicUpdate(r: SuccessorRel, entry: BlockId, n: BlockId, m: seq<BlockId>, cover: set<BlockId>)
+    requires IsAcyclic(r, entry, cover)
+    requires !(n in r.Keys)
+    requires entry != n;
+    requires 
+      forall n1 :: n1 in r.Keys ==>   
+        (forall i :: 0 <= i < |r[n1]| ==> r[n1][i] != n)
+    ensures IsAcyclic(r[n := m], entry, cover)
+  */
+
+  lemma {:verify false} WpCfgUpdate<A(!new)>(a: absval_interp<A>, cfg: Cfg, n: BlockId, source: (BlockId, SimpleCmd), target: seq<BlockId>, post: Predicate<A>, cover: set<BlockId>)
+    requires IsAcyclic(cfg.successors, n, cover)
+    requires cfg.successors.Keys <= cfg.blocks.Keys
+    requires source.0 !in cfg.blocks.Keys
+    requires n != source.0;
+    requires 
+      forall n1 :: n1 in cfg.successors.Keys ==>   
+        (forall i :: 0 <= i < |cfg.successors[n1]| ==> cfg.successors[n1][i] != source.0)
+    ensures 
+      var cfg' := Cfg(cfg.entry, cfg.blocks[source.0 := source.1], cfg.successors[source.0 := target]);
+      WpCfg(a, cfg, n, post, cover) == WpCfg(a, cfg', n, post, cover)
+    {
+      var cfg' := Cfg(cfg.entry, cfg.blocks[source.0 := source.1], cfg.successors[source.0 := target]);
+      var (sourceId, sourceBlock) := source;
+
+      WpCfgExtend2(a, cfg', cfg, map[source.0 := source.1], map[source.0 := target], n, post, cover);
+    }
+
+
+  /*
+
+  lemma {:verify false} IsAcyclicUpdate2(r: SuccessorRel, entry: BlockId, n: BlockId, m: seq<BlockId>, cover: set<BlockId>)
+    requires IsAcyclic(r, entry, cover)
+    requires !(n in r.Keys)
+    requires (forall i :: 0 <= i < |m| ==> ! (m[i] in r.Keys) && !(m[i] ==n))
+    ensures IsAcyclic(r[n := m], entry, cover + {n})
+  */
+
+  lemma {:verify true} WpCfgConjunctionUpdate2<A(!new)>(a: absval_interp<A>, cfg: Cfg, ns: seq<BlockId>, source: BlockId, target: BlockId, post: Predicate<A>, cover: set<BlockId>)
+    requires IsAcyclicSeq(cfg.successors, ns, cover)
+    requires |ns| > 0
+    requires cfg.successors.Keys <= cfg.blocks.Keys
+    requires source in cfg.blocks.Keys
+    requires source !in cfg.successors.Keys
+    requires target !in cfg.blocks.Keys || cfg.blocks[target] == Skip
+    requires target !in cfg.successors.Keys && source != target
+    ensures  WpCfgConjunction(a, cfg, ns, post, cover) ==
+             WpCfgConjunction(a, Cfg(cfg.entry, cfg.blocks[target := Skip], cfg.successors[source := [target]]), ns, post, cover + {source})
+    decreases cover, 1, ns
+    {
+      WpCfgUpdate2(a, cfg, ns[0], source, target, post, cover);
+    }
+
+  lemma {:verify true} WpCfgUpdate2<A(!new)>(a: absval_interp<A>, cfg: Cfg, n: BlockId, source: BlockId, target: BlockId, post: Predicate<A>, cover: set<BlockId>)
+    requires IsAcyclic(cfg.successors, n, cover)
+    requires cfg.successors.Keys <= cfg.blocks.Keys
+    requires source in cfg.blocks.Keys
+    requires source !in cfg.successors.Keys
+    requires target !in cfg.blocks.Keys || cfg.blocks[target] == Skip
+    requires target !in cfg.successors.Keys && source != target
+    ensures  WpCfg(a, cfg, n, post, cover) ==
+             WpCfg(a, Cfg(cfg.entry, cfg.blocks[target := Skip], cfg.successors[source := [target]]), n, post, cover+{source})
+    decreases cover, 0
+  {
+    var cfg' := Cfg(cfg.entry, cfg.blocks[target := Skip], cfg.successors[source := [target]]);
+
+    assert IsAcyclic(cfg'.successors, n, cover + {source}) by {
+      IsAcyclicUpdate2(cfg.successors, n, source, [target], cover);
+    }
+
+
+    if n in cfg.blocks.Keys {
+      var block := cfg.blocks[n];
+      assert block == cfg'.blocks[n];
+
+      if n == source {
+        calc {
+          WpCfg(a, cfg', source, post, cover + {source});
+          WpShallowSimpleCmd(a, block, WpCfgConjunction(a, cfg', [target], post, (cover + {source}) - {source}));
+          WpShallowSimpleCmd(a, block, WpCfg(a, cfg', target, post, (cover + {source}) - {source}));
+          WpShallowSimpleCmd(a, block, post);
+          WpCfg(a, cfg, source, post, cover + {source});
+        }
+      } else {
+        var successors := if n in cfg.successors.Keys then cfg.successors[n] else [];
+
+        if |successors| == 0 {
+
+        } else {
+          WpCfgConjunctionUpdate2(a, cfg, successors, source, target, post, cover - {n});
+          assert (cover-{n})+{source} == (cover+{source})-{n};
+        } 
+      }
+    }
+  }
+
+  lemma {:verify false} IsAcyclicExtendSeq(r1: SuccessorRel, r2: SuccessorRel, ns: seq<BlockId>, cover: set<BlockId>)
+    requires IsAcyclicSeq(r2, ns, cover)
+    requires (forall i :: 0 <= i < |ns| ==> !(ns[i] in r1.Keys))
+    requires 
+      forall n2 :: n2 in r2.Keys ==>   
+        (forall i :: 0 <= i < |r2[n2]| ==> !(r2[n2][i] in r1.Keys))
+    ensures IsAcyclicSeq(r1+r2, ns, cover)
+    decreases cover, 1, ns
+  {
+    if |ns| != 0 {
+      IsAcyclicExtend(r1, r2, ns[0], cover);
+      IsAcyclicExtendSeq(r1, r2, ns[1..], cover);
+    }
+  }
+ 
+  lemma {:verify false} IsAcyclicExtend(r1: SuccessorRel, r2: SuccessorRel, n2Entry: BlockId, cover: set<BlockId>)
+    requires IsAcyclic(r2, n2Entry, cover)
+    requires !(n2Entry in r1.Keys)
+    requires 
+      forall n2 :: n2 in r2.Keys ==>   
+        (forall i :: 0 <= i < |r2[n2]| ==> !(r2[n2][i] in r1.Keys))
+    ensures IsAcyclic(r1+r2, n2Entry, cover)
+    decreases cover, 0
+  {
+    var r := r1 + r2;
+    if(n2Entry in r.Keys) {
+      assert n2Entry in r2.Keys;
+      assert IsAcyclicSeq(r2, r2[n2Entry], cover - {n2Entry});
+
+      IsAcyclicExtendSeq(r1, r2, r2[n2Entry], cover - {n2Entry});
+    }
+  }
+
+  lemma {:verify false} IsAcyclicExtend2(r1: SuccessorRel, r2: SuccessorRel, n1Entry: BlockId, cover: set<BlockId>)
+    requires IsAcyclic(r1, n1Entry, cover)
+    requires !(n1Entry in r2.Keys)
+    requires 
+      forall n1 :: n1 in r1.Keys ==>   
+        (forall i :: 0 <= i < |r1[n1]| ==> !(r1[n1][i] in r2.Keys))
+    requires r1.Keys !! r2.Keys
+    ensures IsAcyclic(r1+r2, n1Entry, cover)
+  {
+    IsAcyclicExtend(r2, r1, n1Entry, cover);
+    assert r2 + r1 == r1 + r2;
+  }
+
+  lemma {:verify false} IsAcyclicUpdate(r: SuccessorRel, entry: BlockId, n: BlockId, m: seq<BlockId>, cover: set<BlockId>)
+    requires IsAcyclic(r, entry, cover)
+    requires !(n in r.Keys)
+    requires entry != n;
+    requires 
+      forall n1 :: n1 in r.Keys ==>   
+        (forall i :: 0 <= i < |r[n1]| ==> r[n1][i] != n)
+    ensures IsAcyclic(r[n := m], entry, cover)
+  {
+    IsAcyclicExtend2(r, map[n := m], entry, cover);
+    assert r+map[n := m] == r[n := m];
+  }
+
+  lemma {:verify false} IsAcyclicSeqOneStep(r: SuccessorRel, ns: seq<BlockId>, cover: set<BlockId>)
+    requires (forall i :: 0 <= i < |ns| ==> ! (ns[i] in r.Keys))
+    ensures IsAcyclicSeq(r, ns, cover)
+  {
+  }
+
+  lemma {:verify false} IsAcyclicSeqUpdate2(r: SuccessorRel, ns: seq<BlockId>, n: BlockId, m: seq<BlockId>, cover: set<BlockId>)
+    requires IsAcyclicSeq(r, ns, cover)
+    requires (forall i :: 0 <= i < |m| ==> ! (m[i] in r.Keys) && !(m[i] == n))
+    ensures IsAcyclicSeq(r[n := m], ns, cover + {n})
+    decreases cover, 1, ns
+  {
+    if |ns| != 0 {
+      IsAcyclicUpdate2(r, ns[0], n, m, cover);
+      IsAcyclicSeqUpdate2(r, ns[1..], n, m, cover);
+    }
+  }
+
+  lemma {:verify false} IsAcyclicUpdate2(r: SuccessorRel, entry: BlockId, n: BlockId, m: seq<BlockId>, cover: set<BlockId>)
+    requires IsAcyclic(r, entry, cover)
+    requires (forall i :: 0 <= i < |m| ==> ! (m[i] in r.Keys) && !(m[i] ==n))
+    ensures IsAcyclic(r[n := m], entry, cover + {n})
+    decreases cover, 0
+  {
+    if(entry == n) {
+      assert IsAcyclic(r[n := m], entry, cover + {n}) by {
+          IsAcyclicSeqOneStep(r[n := m], m, (cover + {n}) - {n});
+      }
+    } else {
+      if entry in r.Keys {
+          IsAcyclicSeqUpdate2(r, r[entry], n, m, cover - {entry}); 
+          assert n != entry;
+          assert (cover - {entry}) + {n} == (cover + {n}) - {entry};
+      }
+    }
+  }
 }
