AstToCfg.dfy
@@ -1,0 +1,181 @@
+include "BoogieLang.dfy"
+include "BoogieSemantics.dfy"
+include "dafny-libraries/src/Wrappers.dfy"
+include "dafny-libraries/src/Math.dfy"
+include "dafny-libraries/src/Collections/Sequences/Seq.dfy"
+
+import opened BoogieLang
+import opened Wrappers
+import opened BoogieSemantics
+import Sequences = Seq
+
+/** 
+  Transforms the Ast `c` into a Cfg.
+  `precedingBlock`: The current basic block that is being processed
+  `currentScope`: Basic block id for current block
+  `labelToBlock`: Basic block ids for all labels in scope
+  `nextVersion`: basic block id that is not reserved (including all ids larger than this one)
+
+  returns:
+    a Cfg if more than one block was completely processed
+    next free version
+    Exit block still under construction (if there is such a block)
+ */
+function method AstToCfgAux(
+  c: Cmd, 
+  precedingBlock: (BlockId, BasicBlock), 
+  currentScope: BlockId, 
+  labelToBlock: map<lbl_name, BlockId>,
+  nextVersion: BlockId) : (Option<Cfg>, BlockId, Option<(BlockId, BasicBlock)>)
+  requires LabelsWellDefAux(c, labelToBlock.Keys)
+  ensures (var res := AstToCfgAux(c, precedingBlock, currentScope, labelToBlock, nextVersion); 
+           var nextVersion' := nextVersion;
+               && (res.0 != None || res.2 != None))
+{
+  match c
+  case SimpleCmd(simpleC) => (None, nextVersion, Some((precedingBlock.0, precedingBlock.1+[simpleC])))
+  case Break(optLbl) =>
+    var succ := if optLbl.Some? then labelToBlock[optLbl.value] else currentScope;
+    var (blockId, block) := precedingBlock;
+    var cfg := Cfg(blockId, map[blockId := block], map[blockId := [succ]]);
+
+    (Some(cfg), nextVersion, None)
+  case Seq(c1, c2) =>
+    var (optCfg1, nextVersion1, optExit1) := AstToCfgAux(c1, precedingBlock, currentScope, labelToBlock, nextVersion);
+
+    if optExit1.None? then
+      //c2 will never be reached
+      (optCfg1, nextVersion1, optExit1)
+    else
+      var (optCfg2, nextVersion2, optExit2) := AstToCfgAux(c2, optExit1.value, currentScope, labelToBlock, nextVersion1);
+
+      if optCfg1.None? then
+        //since the exit block for c1 becomes the preceding block for c2, we can take the result for c2
+        (optCfg2, nextVersion2, optExit2)
+      else if optCfg2.None? then
+        (optCfg1, nextVersion2, optExit2)
+      else
+        //merge cfgs
+        var cfg1 := optCfg1.value;
+        var cfg2 := optCfg2.value;
+        (Some(Cfg(cfg1.entry, cfg1.blocks + cfg2.blocks, cfg1.successors + cfg2.successors)), nextVersion2, optExit2)
+  case If(optCond, c1, c2) => 
+    var (c1StartId, c1StartBlock) := if optCond.Some? then (nextVersion, [Assume(optCond.value)]) else (nextVersion, []);
+    var (c2StartId, c2StartBlock) := if optCond.Some? then (nextVersion+1, [Assume(UnOp(Not, optCond.value))]) else (nextVersion+1, []);
+
+    var (optCfg1, nextVersion1, optExit1) := AstToCfgAux(c1, (c1StartId, c1StartBlock), currentScope, labelToBlock, nextVersion);
+
+    var (optCfg2, nextVersion2, optExit2) := AstToCfgAux(c2, (c2StartId, c2StartBlock), currentScope, labelToBlock, nextVersion1);
+
+    var (entryBlockId, entryBlock) := precedingBlock;
+
+    /** 
+      * precedingBlock is the entry block 
+      * connect precedingBlock to c1StartId and c2StartId
+      * if then/else branch have active exit blocks, then connect those to a fresh basic block, which will became the active basic block
+    */
+
+    var successors1 := if optCfg1.Some? then optCfg1.value.successors else map[];
+    var successors2 := if optCfg2.Some? then successors1 + optCfg2.value.successors else successors1;
+    var successors3 := successors2[entryBlockId := [c1StartId, c2StartId]];
+
+    var blocks1 := if optCfg1.Some? then optCfg1.value.blocks else map[];
+    var blocks2 := if optCfg2.Some? then blocks1 + optCfg2.value.blocks else blocks1;
+    var blocks3 := blocks2[entryBlockId := entryBlock];
+
+    if optExit1.Some? && optExit2.Some? then
+      //connect the end of both branches to a new block
+      var (joinId, joinBlock) := (nextVersion2, []);
+      var (thenExitId, thenExitBlock) := optExit1.value;
+      var (elseExitId, elseExitBlock) := optExit2.value;
+      var successors4 := successors3[thenExitId := [joinId]][elseExitId := [joinId]];
+      var cfg := Cfg(entryBlockId, blocks3, successors3[thenExitId := [joinId]][elseExitId := [joinId]]);
+      (Some(cfg), nextVersion2+1, Some((joinId, joinBlock)))
+    else 
+      var cfg := Cfg(entryBlockId, blocks3, successors3);
+      var optExitResult := if optExit1.Some? then optExit1 else optExit2;
+      (Some(cfg), nextVersion2, optExitResult)
+  case Scope(optLbl, xs, body) => 
+    var (entryBlockId, entryBlock) := precedingBlock;
+    var (lblId, lblBlock) := (nextVersion, []) ;
+
+    var labelToBlockUpd := if optLbl.Some? then labelToBlock[optLbl.value := lblId] else labelToBlock;
+
+    assert labelToBlockUpd.Keys == if optLbl.Some? then {optLbl.value} + labelToBlock.Keys else labelToBlock.Keys;
+    var (optCfg, nextVersion', optExit) := AstToCfgAux(body, (entryBlockId, entryBlock), lblId, labelToBlockUpd, nextVersion+2);
+
+    if optCfg.Some? then
+      var cfg := optCfg.value;
+      if optExit.Some? then
+        var (exitId, exitBlock) := optExit.value;
+        (Some(Cfg(cfg.entry, cfg.blocks[exitId := exitBlock], cfg.successors[exitId := [lblId]])), nextVersion', Some( (lblId, lblBlock) ))
+      else
+        (Some(cfg), nextVersion', Some((lblId, lblBlock)))
+    else
+      var (exitId, exitBlock) := optExit.value;
+
+      (Some(Cfg(entryBlockId, map[lblId := lblBlock, exitId := exitBlock], map[exitId := [lblId]])), nextVersion', Some( (lblId, lblBlock) ))
+  case _ => assume false; (None, nextVersion, None) //TODO
+}
+
+/*
+function ValidCfgAcyclic(g: Cfg, n: BlockId, notVisited: set<BlockId>) : bool
+  requires (n in notVisited)
+  requires CfgWf(g)
+{
+  var successors := g.successors[n];
+  forall i :: 0 <= i < |successors| ==> 
+    ( successors[i] != n && 
+      (successors[i] in notVisited ==> ValidCfgAcyclic(g, n, notVisited - {n}))
+    )
+}
+
+function AcyclicCfg2(g: Cfg, s: set<BlockId>) : bool
+{
+  m.Keys == g.blocks.Keys && 
+  m.Keys == g.successors.Keys &&
+  (forall blockId :: blockId in g.blocks.Keys ==> Sequences.ToSet(g.successors[blockId]) <= m.Keys) &&
+  (forall blockId :: blockId in g.blocks.Keys ==>
+    (forall s :: s in Sequences.ToSet(g.successors[blockId]) ==> m[blockId] < m[s]))
+}
+*/
+ 
+/** termination via topological ordering */
+
+function MaxOfSet(s: set<nat>) : nat
+  ensures (forall i :: i in s ==> MaxOfSet(s) >= i)
+{
+  if s == {} then 0
+  else 
+    var x :| x in s;
+    var subRes := MaxOfSet(s - {x});
+    assert (s - {x}) + {x} == s;
+    Math.Max(subRes, x)
+}
+
+method ForwardTraverse(g: Cfg, n: BlockId, ghost m: map<BlockId, nat>) returns (r: Cfg)
+  requires CfgWf(g)
+  requires n in g.blocks.Keys
+  requires AcyclicCfg(g, m)
+  decreases MaxOfSet(m.Values) - m[n]
+{
+  assert m[n] in m.Values;
+  var i := 0;
+  while (i < |g.successors[n]|)
+  { 
+    var suc := g.successors[n][i];
+    reveal Sequences.ToSet();
+    r := ForwardTraverse(g, g.successors[n][i], m);
+    i := i+1;
+  }
+}
+
+function AcyclicCfg(g: Cfg, m: map<BlockId, nat>) : bool
+{
+  m.Keys == g.blocks.Keys && 
+  m.Keys == g.successors.Keys &&
+  (forall blockId :: blockId in g.blocks.Keys ==> Sequences.ToSet(g.successors[blockId]) <= m.Keys) &&
+  (forall blockId :: blockId in g.blocks.Keys ==>
+    (forall s :: s in Sequences.ToSet(g.successors[blockId]) ==> m[blockId] < m[s]))
+}
+
