AstToCfg_simple.dfy
@@ -1,0 +1,267 @@
+include "Cfg.dfy"
+include "dafny-libraries/src/Wrappers.dfy"
+include "dafny-libraries/src/Math.dfy"
+include "dafny-libraries/src/Collections/Sequences/Seq.dfy"
+
+module AstToCfg {
+
+  import opened BoogieLang
+  import opened Wrappers
+  import opened BoogieSemantics
+  import Sequences = Seq
+  import opened BoogieCfg
+  import Math
+
+  predicate NoBreaksScopedVarsLoops(c: Cmd)
+  {
+    match c
+    case SimpleCmd(_) => true
+    case Break(optLbl) => false
+    case Seq(thn, els) => NoBreaksScopedVarsLoops(thn) && NoBreaksScopedVarsLoops(els)
+    case Loop(_,_) => false
+    case Scope(_, varDecls, body) => varDecls == [] && NoBreaksScopedVarsLoops(body)
+    case If(_, thn, els) => NoBreaksScopedVarsLoops(thn) && NoBreaksScopedVarsLoops(els)
+  }
+
+  function {:opaque} CoveringSet(oldVersion: nat, newVersion: nat, exclude: nat) : set<nat>
+  {
+    (set x : nat | oldVersion <= x < newVersion) - {exclude}
+  }
+
+  /** 
+    Transforms the Ast `c` into a Cfg.
+    `nextVersion`: basic block id that is not reserved (including all ids larger than this one)
+
+    returns:
+      a cfg 
+      next free version
+      exit block of returned cfg 
+  */
+  function method AstToCfgAux(c: Cmd, nextVersion: BlockId) : (Cfg, BlockId, Option<BlockId>) 
+    //Option for exit block needed once break statements are taken into account
+    requires NoBreaksScopedVarsLoops(c)
+    ensures  var (cfg, nextVersion', exitOpt):= AstToCfgAux(c, nextVersion); 
+                exitOpt != None  &&
+                var exit := exitOpt.value;
+                && cfg.successors.Keys == cfg.blocks.Keys - {exit}
+                && nextVersion < nextVersion' 
+                && (nextVersion <= exit < nextVersion')
+                && (forall n :: n in cfg.blocks.Keys ==> nextVersion <= n < nextVersion')
+                && cfg.entry in cfg.blocks.Keys
+                && exit in cfg.blocks.Keys
+                   //exit block is the only sink block (note that exit block is not in successors.Keys)
+                && (forall n :: n in cfg.successors.Keys ==> cfg.successors[n] != []) 
+  {
+    match c
+    case SimpleCmd(simpleC) =>
+      (Cfg(nextVersion, map[nextVersion := simpleC], map[]), nextVersion+1, Some(nextVersion))
+    case Seq(c1, c2) =>
+      var (cfg1, nextVersion1, exitOpt1) := AstToCfgAux(c1, nextVersion);
+      if exitOpt1.None? then
+        //c2 will never be reached
+        (cfg1, nextVersion1, exitOpt1)
+      else 
+        var (cfg2, nextVersion2, exitOpt2) := AstToCfgAux(c2, nextVersion1);
+
+        var blocks := cfg1.blocks + cfg2.blocks;
+        var successors := (cfg1.successors + cfg2.successors)[exitOpt1.value := [cfg2.entry]];
+  
+        (Cfg(cfg1.entry, cfg1.blocks + cfg2.blocks, successors), nextVersion2, exitOpt2)
+    case Scope(_, varDecls, body) =>
+      // scoped variable declarations have been compiled away
+      assert varDecls == [];
+
+      /* since our precondition ensures that there are no breaks, we need not 
+      worry about jumps out of this scope and can just return the result for the 
+      body (TODO: lift the precondition) */
+
+      AstToCfgAux(body, nextVersion)
+
+    case If(optCond, thn, els) => 
+      /** CFG thn branch */
+      var (entryId, entryBlock) := (nextVersion, Skip);
+      var (cfgThn, nextVersion1, exitOpt1) := AstToCfgAux(thn, entryId+1);
+
+      var cfgThn' := 
+        if optCond.Some? then
+          Cfg(cfgThn.entry, cfgThn.blocks[cfgThn.entry := SeqSimple(Assume(optCond.value), cfgThn.blocks[cfgThn.entry])], cfgThn.successors)
+        else
+          cfgThn;
+
+      /** CFG els branch */
+      var (cfgEls, nextVersion2, exitOpt2) := AstToCfgAux(els, nextVersion1);
+
+      var cfgEls' := 
+        if optCond.Some? then
+          Cfg(cfgEls.entry, cfgEls.blocks[cfgEls.entry := SeqSimple(Assume(UnOp(Not, optCond.value)), cfgEls.blocks[cfgEls.entry])], cfgEls.successors)
+        else
+          cfgEls;
+
+      /** 
+        * connect entry block to thnStartId and elsStartId
+        * if then/else branch have active exit blocks, then connect those to a fresh basic block, which will became the active basic block
+      */
+
+      /** new successor relation */
+      var (blocksThnEls, successorsThnEls) := 
+        (cfgThn'.blocks + cfgEls'.blocks, cfgThn'.successors + cfgEls'.successors);
+
+      var blocksBeforeJoin := blocksThnEls[entryId := entryBlock]; 
+      var successorsBeforeJoin := successorsThnEls[entryId := [cfgThn'.entry, cfgEls'.entry]];
+
+      if exitOpt1.Some? && exitOpt2.Some? then
+        //connect the end of both branches to a new block
+        var (joinId, joinBlock) := (nextVersion2, Skip);
+        var thnExit := exitOpt1.value;
+        var elsExit := exitOpt2.value;
+
+        var blocks := blocksBeforeJoin[joinId := joinBlock];
+        var successors := successorsBeforeJoin[thnExit := [joinId]][elsExit := [joinId]];
+        var cfg := Cfg(entryId, blocks, successors);
+
+        (cfg, nextVersion2+1, Some(joinId))
+      else 
+        var cfg := Cfg(entryId, blocksBeforeJoin, successorsBeforeJoin);
+        var exitOptResult := if exitOpt1.Some? then exitOpt1 else exitOpt2;
+        (cfg, nextVersion2, exitOptResult)
+  }
+
+  lemma AstToCfgAcyclic(
+    c: Cmd, 
+    nextVersion: BlockId)
+    requires NoBreaksScopedVarsLoops(c)
+    ensures  
+      var (cfg, nextVersion', exitOpt):= AstToCfgAux(c, nextVersion); 
+
+      var exit := exitOpt.value;
+      var s := cfg.successors;
+      
+      && (forall n :: n in s.Keys ==>   
+          (forall i :: 0 <= i < |s[n]| ==> (s[n][i] == exit || s[n][i] in s.Keys))) 
+      && cfg.entry in cfg.blocks.Keys 
+      && IsAcyclic(cfg.successors, cfg.entry, CoveringSet(nextVersion, nextVersion', exit))
+  {
+    match c {
+      case SimpleCmd(sc) =>  
+      case Seq(c1, c2) =>
+        var (cfg1, nextVersion1, exitOpt1) := AstToCfgAux(c1, nextVersion);
+        var exit1 := exitOpt1.value;
+        assert IsAcyclic(cfg1.successors, cfg1.entry, CoveringSet(nextVersion, nextVersion1, exit1));
+
+        var (cfg2, nextVersion2, exitOpt2) := AstToCfgAux(c2, nextVersion1);
+        AstToCfgAcyclic(c2, nextVersion2);
+
+        var exit2 := exitOpt2.value;
+
+        //merge cfgs
+
+        var cover1 := CoveringSet(nextVersion, nextVersion1, exit1);
+        var cover2 := CoveringSet(nextVersion1, nextVersion2, exit2);
+        var cover3 := CoveringSet(nextVersion, nextVersion2, exit2);
+
+
+        var successors := (cfg1.successors + cfg2.successors)[exitOpt1.value := [cfg2.entry]];
+        assert successors == (cfg1.successors[exitOpt1.value := [cfg2.entry]] + cfg2.successors);
+
+        assert cover1 !! cover2 by {
+          reveal CoveringSet();
+        }
+        assert cfg1.successors.Keys !! cfg2.successors.Keys;
+
+        IsAcyclicUpdate2(cfg1.successors, cfg1.entry, exit1, [cfg2.entry], cover1);
+
+        assert IsAcyclic(cfg1.successors[exit1 := [cfg2.entry]], cfg1.entry, cover1+{exit1});
+
+        assert (cover1+{exit1} !! cover2) by {
+          reveal CoveringSet();
+        }
+
+        IsAcyclicMerge(
+          cfg1.successors[exit1 := [cfg2.entry]], cfg2.successors, cfg1.entry, cfg2.entry, 
+          cover1+{exit1},
+          cover2
+          );
+
+        assert (cover1 + {exit1}) + cover2 <= cover3 by {
+          reveal CoveringSet();
+        }
+        IsAcyclicLargerCover(successors, cfg1.entry, (cover1 + {exit1}) + cover2, cover3);
+      case Scope(_, varDecls, body) => 
+      case If(optCond, thn, els) => 
+        /** CFG thn branch */
+        var (entryId, entryBlock) := (nextVersion, Skip);
+        var (cfgThn, nextVersion1, exitOpt1) := AstToCfgAux(thn, entryId+1);
+
+        var cfgThn' := 
+          if optCond.Some? then
+            Cfg(cfgThn.entry, cfgThn.blocks[cfgThn.entry := SeqSimple(Assume(optCond.value), cfgThn.blocks[cfgThn.entry])], cfgThn.successors)
+          else
+            cfgThn;
+
+        /** CFG els branch */
+        var (cfgEls, nextVersion2, exitOpt2) := AstToCfgAux(els, nextVersion1);
+
+        var cfgEls' := 
+          if optCond.Some? then
+            Cfg(cfgEls.entry, cfgEls.blocks[cfgEls.entry := SeqSimple(Assume(UnOp(Not, optCond.value)), cfgEls.blocks[cfgEls.entry])], cfgEls.successors)
+          else
+            cfgEls;
+
+        var (entry1, s1) := (cfgThn.entry, cfgThn.successors);
+        var thnExit := exitOpt1.value;
+
+        var cover1 := CoveringSet(nextVersion+1, nextVersion1, thnExit);
+        assert IsAcyclic(s1, entry1, cover1);
+
+        var (entry2, s2) := (cfgEls.entry, cfgEls.successors);
+        var elsExit := exitOpt2.value;
+
+        var cover2 := CoveringSet(nextVersion1, nextVersion2, elsExit);
+        assert IsAcyclic(s2, entry2, cover2);
+
+        IsAcyclicExtend2(s1, s2, entry1, cover1);
+        IsAcyclicLargerCover(s1 + s2, entry1, cover1, cover1+cover2);
+        assert IsAcyclic(s1 + s2, entry1, cover1+cover2);
+
+        IsAcyclicExtend(s1, s2, entry2, cover2);
+        IsAcyclicLargerCover(s1 + s2, entry2, cover2, cover1+cover2);
+        assert IsAcyclic(s1 + s2, entry2, cover1+cover2);
+
+        var successorsBeforeJoin := (s1 + s2)[entryId := [cfgThn'.entry, cfgEls'.entry]];
+
+        assert IsAcyclic(successorsBeforeJoin, entryId, cover1+cover2+{entryId}) by {
+          calc {
+            IsAcyclic(successorsBeforeJoin, entryId, cover1+cover2+{entryId});
+            { reveal CoveringSet(); }
+            IsAcyclicSeq(successorsBeforeJoin, [cfgThn'.entry, cfgEls'.entry], cover1+cover2);
+            IsAcyclic(successorsBeforeJoin, cfgThn'.entry, cover1+cover2) &&
+            IsAcyclicSeq(successorsBeforeJoin, [cfgEls'.entry], cover1+cover2);
+            IsAcyclic(successorsBeforeJoin, cfgThn'.entry, cover1+cover2) &&
+            IsAcyclic(successorsBeforeJoin, cfgEls'.entry, cover1+cover2);
+            { IsAcyclicUpdate(s1+s2, entry1, entryId, [cfgThn'.entry, cfgEls'.entry], cover1+cover2);
+              IsAcyclicUpdate(s1+s2, entry2, entryId, [cfgThn'.entry, cfgEls'.entry], cover1+cover2);
+            }
+            IsAcyclic(s1+s2, cfgThn'.entry, cover1+cover2) &&
+            IsAcyclic(s1+s2, cfgEls'.entry, cover1+cover2);
+          }
+        }
+
+        IsAcyclicUpdate2(successorsBeforeJoin, entryId, thnExit, [nextVersion2], cover1+cover2+{entryId});
+        IsAcyclicUpdate2(successorsBeforeJoin[thnExit := [nextVersion2]], entryId, elsExit, [nextVersion2], cover1+cover2+{entryId}+{thnExit});
+
+        var successorsBeforeJoinImpl := (s1+s2)[entryId := [cfgThn'.entry, cfgEls'.entry]];
+
+        var successors := successorsBeforeJoinImpl[thnExit := [nextVersion2]][elsExit := [nextVersion2]];
+        var cover3 := cover1+cover2+{entryId}+{thnExit}+{elsExit};
+
+        assert IsAcyclic(successors, entryId, cover3) by {
+          assert successors == successorsBeforeJoin[thnExit := [nextVersion2]][elsExit := [nextVersion2]];
+        }
+        
+        assert IsAcyclic(successors, entryId, CoveringSet(nextVersion, nextVersion2+1, nextVersion2)) by {
+          reveal CoveringSet();
+          assert cover3 == CoveringSet(nextVersion, nextVersion2+1, nextVersion2);
+        }
+    }
+  }           
+}
