CfgMisc.dfy
@@ -1,0 +1,166 @@
+
+  include "Cfg.dfy"
+
+  module CfgMisc {
+    import opened BoogieLang
+    import opened BoogieSemantics
+    import opened Wrappers
+    import opened BoogieCfg
+
+
+  lemma WpCfgConjunctionSingle<A(!new)>(
+    a: absval_interp<A>, 
+    g: Cfg, 
+    ns: seq<BlockId>, 
+    n: BlockId,
+    post: Predicate<A>, 
+    cover: set<BlockId>,
+    s: state<A>) 
+  requires g.blocks.Keys == g.successors.Keys
+  requires IsAcyclic(g.successors, n, cover)
+  requires IsAcyclicSeq(g.successors, ns, cover)
+  requires n in ns
+  ensures  var nPre := WpCfg(a, g, n, post, cover)(s);
+           var nsPre := WpCfgConjunction(a, g, ns, post, cover)(s);
+           ImpliesOpt(nsPre, nPre)
+  /** TODO proof */
+
+  /*============================Wp with acyclicity============================*/
+  function WpCfgConjunctionAcyclic<A(!new)>(
+    a: absval_interp<A>, 
+    g: Cfg, 
+    ns: seq<BlockId>, 
+    post: Predicate<A>, 
+    cover: set<BlockId>) : Predicate<A>
+    requires g.successors.Keys <= g.blocks.Keys //not being in the domain of the successor relation is the same as not having any successors
+    requires IsAcyclicSeq(g.successors, ns, cover)
+    decreases cover, 1, ns
+  { s =>
+      if |ns| == 0 then Some(true)
+      else 
+        var res1 :- WpCfg(a, g, ns[0], post, cover)(s);
+        var res2 :- WpCfgConjunction(a, g, ns[1..], post, cover)(s);
+        Some(res1 && res2)
+  }
+
+  function WpCfgAcyclic<A(!new)>(a: absval_interp<A>, g: Cfg, n: BlockId, post: Predicate<A>, cover: set<BlockId>) : Predicate<A>
+    requires g.successors.Keys <= g.blocks.Keys //not being in the domain of the successor relation is the same as not having any successors
+    requires IsAcyclic(g.successors, n, cover)
+    decreases cover, 0
+  {
+    if n !in g.blocks.Keys then
+      post
+    else 
+      var successors := if n in g.successors.Keys then g.successors[n] else [];
+      if |successors| == 0 then 
+        WpShallowSimpleCmd(a, g.blocks[n], post)
+      else 
+        WpShallowSimpleCmd(a, g.blocks[n], WpCfgConjunction(a, g, successors, post, cover - {n}))
+  }
+
+  lemma WpCfgConjunctionAcyclicEquiv<A(!new)>(a: absval_interp<A>, g: Cfg, ns: seq<BlockId>, post: Predicate<A>, cover: set<BlockId>)
+    requires g.successors.Keys <= g.blocks.Keys 
+    requires IsAcyclicSeq(g.successors, ns, cover)
+    ensures WpCfgConjunction(a, g, ns, post, cover) == WpCfgConjunctionAcyclic(a, g, ns, post, cover)
+    decreases cover, 1, ns
+
+  lemma WpCfgAcyclicEquiv<A(!new)>(a: absval_interp<A>, g: Cfg, n: BlockId, post: Predicate<A>, cover: set<BlockId>)
+    requires g.successors.Keys <= g.blocks.Keys //not being in the domain of the successor relation is the same as not having any successors
+    requires IsAcyclic(g.successors, n, cover)
+    ensures WpCfg(a, g, n, post, cover) == WpCfgAcyclic(a, g, n, post, cover)
+    decreases cover, 0
+  {
+    var successors := if n in g.successors.Keys then g.successors[n] else [];
+    if |successors| != 0 {
+      WpCfgConjunctionAcyclicEquiv(a, g, successors, post, cover - {n});
+    }
+  }
+
+    
+  /*============================Operational semantics========================*/
+
+  least predicate CfgRed<A(!new)>(a: absval_interp<A>, g: Cfg, n: BlockId, s: ExtState<A>, s': ExtState<A>)
+    requires g.blocks.Keys == g.successors.Keys
+  {
+    if n in g.blocks.Keys then
+      var blocks := g.blocks[n];
+      var successors := g.successors[n];
+
+      if |successors| == 0 then
+        SimpleCmdOpSem(a, blocks, s, s')
+      else
+        assert successors[0] in successors; //required for non-emptiness constraint in next line to go through
+        var succ :| succ in successors;
+        (exists s'' :: SimpleCmdOpSem(a, blocks, s, s'') && CfgRed(a, g, succ, s'' , s'))
+    else 
+      false
+  }
+
+/*==========Correspondence Wp and Operational Semantics===========================*/
+
+  lemma WpSemToOpSem_SimpleCmd<A(!new)>(a: absval_interp<A>, scs: SimpleCmd, post: Predicate<A>, s: state<A>, s': ExtState<A>)
+    requires WpShallowSimpleCmd(a, scs, post)(s) == Some(true)
+    requires SimpleCmdOpSem(a, scs, NormalState(s), s')
+    ensures s' != FailureState
+    ensures forall ns' :: s' == NormalState(ns') ==> post(ns') == Some(true)
+  /** TODO proof */
+ 
+  //Note that the following lemma is trivially satisfied if CfgRed is the empty relation
+  lemma WpSemToOpSem<A(!new)>(a: absval_interp<A>, g: Cfg, n: BlockId, post: Predicate<A>, cover: set<BlockId>, s: state<A>, s': ExtState<A>)
+    requires IsAcyclic(g.successors, n, cover)
+    requires g.successors.Keys == g.blocks.Keys
+    requires WpCfg(a, g, n, post, cover)(s) == Some(true)
+    requires CfgRed(a, g, n, NormalState(s), s')
+    requires CfgWf(g) && n in g.blocks.Keys
+    ensures s' != FailureState
+    ensures forall ns' :: s' == NormalState(ns') ==> post(ns') == Some(true)
+    decreases cover
+  {
+    var block := g.blocks[n];
+    var successors := g.successors[n];
+
+    if |successors| == 0 {
+      WpSemToOpSem_SimpleCmd(a, block, post, s, s');
+    } else {
+      assert WpShallowSimpleCmd(a, block, WpCfgConjunction(a, g, successors, post, cover - {n}))(s) == Some(true);
+
+      var succ, y :| succ in successors && SimpleCmdOpSem(a, block, NormalState(s), y) && CfgRed(a, g, succ, y , s');
+
+      WpSemToOpSem_SimpleCmd(a, block, WpCfgConjunction(a, g, successors, post, cover - {n}), s, y);
+
+      match y {
+        case MagicState => assume false; //TODO magic state stays magic
+        case NormalState(s'') => 
+        calc {
+          IsAcyclic(g.successors, n, cover);
+          ==>
+          IsAcyclicSeq(g.successors, successors, cover - {n});
+          ==> { IsAcyclicElem(g.successors, successors, succ, cover - {n}); }
+          IsAcyclic(g.successors, succ, cover - {n});
+        }
+        assert WpCfg(a, g, succ, post, cover - {n})(s'') == Some(true) by {
+          WpCfgConjunctionSingle(a, g, successors, succ, post, cover - {n}, s'');
+        }
+        
+        WpSemToOpSem(a, g, succ, post, cover - {n}, s'', s');
+      }
+    }
+  }
+
+  /** TODO OpSem to WP */
+  function CfgRedSet<A(!new)>(a: absval_interp<A>, g: Cfg, n: BlockId, y: ExtState<A>) : iset<ExtState<A>>
+    requires g.blocks.Keys == g.successors.Keys
+  {
+    iset y' | CfgRed(a, g, n, y, y')
+  }
+
+  lemma OpSemToWpSem<A(!new)>(a: absval_interp<A>, g: Cfg, n: BlockId, post: Predicate<A>, cover: set<BlockId>, s: state<A>)
+    requires IsAcyclic(g.successors, n, cover)
+    requires g.successors.Keys == g.blocks.Keys
+    requires !(FailureState in CfgRedSet(a, g, n, NormalState(s)))
+    requires CfgWf(g) && n in g.blocks.Keys
+    ensures var wpRes := WpCfg(a, g, n, s' => Some(NormalState(s') in CfgRedSet(a, g, n, NormalState(s))), cover)(s);
+            wpRes == Some(true) || wpRes == None
+    decreases cover
+  /** TODO: proof */
+}
