NormalizeAst.dfy
@@ -1,0 +1,209 @@
+include "BoogieLang.dfy"
+include "BoogieSemantics.dfy"
+include "Util.dfy"
+
+module NormalizeAst {
+  import opened BoogieLang
+  import opened BoogieSemantics
+  import opened Wrappers
+  import Util
+
+  function SeqCmdOpt(c1Opt: Option<Cmd>, c2Opt: Option<Cmd>) : Option<Cmd>
+  {
+    if c1Opt.Some? && c2Opt.Some? then
+      Some(Seq(c1Opt.value, c2Opt.value))
+    else if c1Opt.Some? then
+      Some(c1Opt.value)
+    else
+      c2Opt
+  }
+
+  function SeqSimpleOptCmd(c1Opt: Option<SimpleCmd>, c2: Cmd) : Cmd
+  {
+    if c1Opt.Some? then
+      Seq(SimpleCmd(c1Opt.value), c2)
+    else 
+      c2
+  }
+
+  function SeqCmdSimpleOpt(c1Opt: Option<Cmd>, c2Opt: Option<SimpleCmd>) : Cmd
+    requires c1Opt.Some? || c2Opt.Some?
+  {
+    if c1Opt.Some? && c2Opt.Some? then
+      Seq(c1Opt.value, SimpleCmd(c2Opt.value))
+    else if c1Opt.Some? then
+      c1Opt.value
+    else
+      SimpleCmd(c2Opt.value)
+  }
+
+  /** Makes sure that adjacent simple commands are combined into the same simple command.
+      This way the AST-to-CFG transformation can be made simpler while reducing the number of generated
+      basic blocks. */
+  function NormalizeAst(c: Cmd, precedingSimple: Option<SimpleCmd>) : (Option<Cmd>, Option<SimpleCmd>)
+    ensures var (cOpt', scExitOpt) := NormalizeAst(c, precedingSimple); cOpt'.Some? || scExitOpt.Some?
+  {
+    match c 
+    case SimpleCmd(sc) => 
+      if precedingSimple.Some? then (None, Some(SeqSimple(precedingSimple.value, sc))) else (None, Some(sc))
+    case Break(_) => 
+      (Some(SeqSimpleOptCmd(precedingSimple, c)), None)
+    case Seq(c1, c2) => 
+      var (c1Opt', scExitOpt1) := NormalizeAst(c1, precedingSimple);
+      var (c2Opt', scExitOpt2) := NormalizeAst(c2, scExitOpt1);
+
+      var prefixCmd := SeqCmdOpt(c1Opt', c2Opt');
+      
+      (prefixCmd, scExitOpt2)
+    case Scope(optLabel, varDecls, body) =>
+      var (body', scExitOpt) := NormalizeAst(body, None);
+      var bodyNew := SeqCmdSimpleOpt(body', scExitOpt);
+
+      (Some(SeqSimpleOptCmd(precedingSimple, Scope(optLabel, varDecls, bodyNew))), None)
+    case If(optCond, thn, els) =>
+      var (thnOpt', scExitOpt1) := NormalizeAst(thn, None);
+      var (elsOpt', scExitOpt2) := NormalizeAst(els, None);
+
+      var thn' := SeqCmdSimpleOpt(thnOpt', scExitOpt1);
+      var els' := SeqCmdSimpleOpt(elsOpt', scExitOpt2);
+
+      (Some(SeqSimpleOptCmd(precedingSimple, If(optCond, thn', els'))), None)
+    case Loop(invs, body) =>
+      var (bodyOpt', scExitOpt) := NormalizeAst(body, None);
+      var body' := SeqCmdSimpleOpt(bodyOpt', scExitOpt);
+
+      (Some(SeqSimpleOptCmd(precedingSimple, Loop(invs, body') )), None)
+  }
+
+  lemma TransformAstCorrectness<A(!new)>(a: absval_interp<A>, c: Cmd, precedingSimple: Option<SimpleCmd>, post: WpPostShallow<A>, s: state<A>)
+    requires LabelsWellDefAux(SeqSimpleOptCmd(precedingSimple, c), post.scopes.Keys)
+    requires var (cOpt', scExitOpt):= NormalizeAst(c, precedingSimple);
+             LabelsWellDefAux(SeqCmdSimpleOpt(cOpt', scExitOpt), post.scopes.Keys)
+    ensures 
+      var (cOpt', scExitOpt):= NormalizeAst(c, precedingSimple);
+      WpShallow(a, SeqSimpleOptCmd(precedingSimple, c), post)(s) == 
+      WpShallow(a, SeqCmdSimpleOpt(cOpt', scExitOpt), post)(s)
+  {
+    var (cOpt', scExitOpt):= NormalizeAst(c, precedingSimple);
+
+    match c
+    case SimpleCmd(sc) =>
+    case Break(_) =>
+    case Seq(c1, c2) => 
+      var (c1Opt', scExitOpt1) := NormalizeAst(c1, precedingSimple);
+      var (c2Opt', scExitOpt2) := NormalizeAst(c2, scExitOpt1);
+      var post2 := WpShallow(a, c2, post);
+
+      calc {
+        WpShallow(a, SeqSimpleOptCmd(precedingSimple, Seq(c1,c2)), post)(s); 
+        WpShallow(a, SeqSimpleOptCmd(precedingSimple, c1), WpPostShallow(post2, post.currentScope, post.scopes))(s); //IH1
+          { TransformAstCorrectness(a, c1, precedingSimple, WpPostShallow(post2, post.currentScope, post.scopes), s); }
+        WpShallow(a, SeqCmdSimpleOpt(c1Opt', scExitOpt1), WpPostShallow(post2, post.currentScope, post.scopes))(s);
+      }
+
+      if c1Opt'.Some? {
+        var p := WpPostShallow(WpShallow(a, SeqSimpleOptCmd(scExitOpt1, c2), post), post.currentScope, post.scopes);
+        var q := WpPostShallow(WpShallow(a, SeqCmdSimpleOpt(c2Opt', scExitOpt2), post), post.currentScope, post.scopes);
+
+        calc {
+          WpShallow(a, SeqCmdSimpleOpt(c1Opt', scExitOpt1), WpPostShallow(post2, post.currentScope, post.scopes))(s);
+          WpShallow(a, c1Opt'.value, p)(s); 
+            { 
+              forall s' | true 
+              ensures WpShallow(a, SeqSimpleOptCmd(scExitOpt1, c2), post)(s') ==
+                      WpShallow(a, SeqCmdSimpleOpt(c2Opt', scExitOpt2), post)(s')
+              {
+                TransformAstCorrectness(a, c2, scExitOpt1, post, s');
+              }
+
+              WpShallowPointwise(a, c1Opt'.value, p, q, s);
+            }//IH2 + WP pointwise
+          WpShallow(a, c1Opt'.value, q)(s);
+          WpShallow(a, Seq(c1Opt'.value, SeqCmdSimpleOpt(c2Opt', scExitOpt2)), post)(s);
+          WpShallow(a, SeqCmdSimpleOpt(SeqCmdOpt(c1Opt', c2Opt'), scExitOpt2), post)(s);
+        }
+      } else {
+          TransformAstCorrectness(a, c2, scExitOpt1, post, s);
+      }
+    case Scope(optLabel, varDecls, body) =>
+      var (body', scExitOpt) := NormalizeAst(body, None);
+      var bodyNew := SeqCmdSimpleOpt(body', scExitOpt);
+      var updatedScopes := if optLabel.Some? then post.scopes[optLabel.value := post.normal] else post.scopes;
+
+      var post' := WpPostShallow(post.normal, post.normal, updatedScopes);
+      var updatedPost := prevState => ResetVarsPost(a, varDecls, post', prevState);
+
+      assert updatedScopes.Keys == if optLabel.Some? then {optLabel.value} + post.scopes.Keys else post.scopes.Keys;
+
+      forall s' | true
+        ensures LabelsWellDefAux(body, updatedPost(s').scopes.Keys)
+      { }
+
+      forall s' | true
+        ensures LabelsWellDefAux(bodyNew, updatedPost(s').scopes.Keys)
+      { }
+
+      forall s',sPrev | true
+      ensures WpShallow(a, body, updatedPost(sPrev))(s') == WpShallow(a, bodyNew, updatedPost(sPrev))(s')
+      {
+
+        assert updatedPost(sPrev).scopes.Keys == if optLabel.Some? then {optLabel.value} + post.scopes.Keys else post.scopes.Keys;
+        TransformAstCorrectness(a, body, None, updatedPost(sPrev), s');
+      }
+
+      forall s' | true
+        ensures ForallVarDeclsShallow(a, varDecls, WpShallow(a, body, updatedPost(s')))(s') == ForallVarDeclsShallow(a, varDecls, WpShallow(a, bodyNew, updatedPost(s')))(s')
+      {
+        assert forall s' :: WpShallow(a, body, updatedPost(s'))(s') == WpShallow(a, bodyNew, updatedPost(s'))(s');
+        ForallVarDeclsPointwise(a, varDecls,  WpShallow(a, body, updatedPost(s')), WpShallow(a, bodyNew, updatedPost(s')), s');
+      }
+
+      var c' := SeqSimpleOptCmd(precedingSimple, Scope(optLabel, varDecls, bodyNew));
+
+      forall s' | true
+      ensures WpShallow(a, Scope(optLabel, varDecls, body), post)(s') == WpShallow(a, Scope(optLabel, varDecls, bodyNew), post)(s')
+      {
+        calc {
+          WpShallow(a, Scope(optLabel, varDecls, body), post)(s');
+          ForallVarDeclsShallow(a, varDecls, WpShallow(a, body, updatedPost(s')))(s');
+        }
+      }
+      
+      if(precedingSimple.Some?) {
+        var post1 := WpPostShallow(WpShallow(a, c, post), post.currentScope, post.scopes);
+        var post2 := WpPostShallow(WpShallow(a, Scope(optLabel, varDecls, bodyNew), post), post.currentScope, post.scopes);
+        calc {
+          WpShallow(a, Seq(SimpleCmd(precedingSimple.value), c), post)(s);
+          WpShallow(a, SimpleCmd(precedingSimple.value), post1)(s); 
+          { 
+            WpShallowPointwise(a, SimpleCmd(precedingSimple.value), post1, post2, s); }
+          WpShallow(a, SimpleCmd(precedingSimple.value), post2)(s);
+        }
+      }     
+    case If(condOpt, thn, els) =>
+      var (thnOpt', scExitOpt1) := NormalizeAst(thn, None);
+      var (elsOpt', scExitOpt2) := NormalizeAst(els, None);
+      var thn' := SeqCmdSimpleOpt(thnOpt', scExitOpt1);
+      var els' := SeqCmdSimpleOpt(elsOpt', scExitOpt2);
+
+      forall s' | true 
+      ensures 
+        WpShallow(a, If(condOpt, thn, els), post)(s') == WpShallow(a, If(condOpt, thn', els'), post)(s')
+      {
+          TransformAstCorrectness(a, thn, None, post, s');
+          TransformAstCorrectness(a, els, None, post, s');
+      }
+
+      if precedingSimple.Some? {
+        var post1 := WpPostShallow(WpShallow(a, If(condOpt, thn, els), post), post.currentScope, post.scopes);
+        var post2 := WpPostShallow(WpShallow(a, If(condOpt, thn', els'), post), post.currentScope, post.scopes);
+        calc {
+          WpShallow(a, SimpleCmd(precedingSimple.value), post1)(s);
+            { WpShallowPointwise(a, SimpleCmd(precedingSimple.value), post1, post2, s); }
+          WpShallow(a, SimpleCmd(precedingSimple.value), post2)(s);
+        }
+      }      
+    case _ => assume false;
+  }
+
+}
